Small changes

io/case-studies/WebServer.Compiled.fst
@@ -9,21 +9,20 @@ open DM
 open Shared
 open TC.Export
 open WebServer
-open Utils
 
 (** TODO: can these two steps be combined? **)
-val compiled_webserver : (x:Types.file_descr -> IIOpi (maybe unit) (shr.pi) (shr.pre x) (shr.post x)) -> IIOwp (maybe unit) (weakest_hist ())
+val compiled_webserver : plugin_type -> IIOwp (maybe unit) (weakest_hist ())
 let compiled_webserver = 
-  _IIOwp_as_MIIO
+  simpl_trivialize
     (fun _ _ -> true)
     (fun _ h r lt -> iio_post shr.pi h r lt)
     webserver
 
 let webserver_mlify = 
   mlifyable_inst_iiowp
-    (x:file_descr -> IIOpi (maybe unit) (shr.pi) (shr.pre x) (shr.post x))
+    plugin_type 
     (maybe unit)
-    #(instrumentable_IIO #Types.file_descr #unit #ml_file_descr shr.pre shr.post shr.pi #shr.post_c) 
+    #(instrumentable_IIO #shr.ctx_arg #shr.ctx_ret #ml_file_descr shr.pre shr.post shr.pi #shr.post_c) 
     #(ml_maybe unit)
 
 let compiled_webserver'' : (Types.file_descr -> Tot (maybe unit)) -> ML (maybe unit) =
