io/case-studies/Utils.fst
@@ -44,7 +44,7 @@ effect IOpi
       pre h /\
       (forall r lt. (io_post pi h r lt /\ post h r lt) ==> p lt r))
 
-let _IIOwp_as_MIIO
+let simpl_trivialize 
   (pre:'a -> trace -> bool)
   (post:'a -> trace -> (m:'b) -> trace -> Type0)
   (f:(x:'a ->
@@ -54,14 +54,3 @@ let _IIOwp_as_MIIO
   (trivialize 
     #_ 
     #(trivializeable_IIOwp _ _ (fun x h -> pre x h) post) f) x
-
-let _IIOwp_as_MIIO_2
-  (pre:'a -> 'b -> trace -> bool)
-  (post:'a -> 'b -> trace -> (m:'c) -> trace -> Type0)
-  (f:(x:'a -> y:'b ->
-    IIOwp 'c (fun p h -> pre x y h /\ (forall r lt. post x y h r lt ==> p lt r))))
-  (x:'a) (y:'b):
-  IIOwp (Common.maybe 'c) (weakest_hist ()) =
-  (trivialize 
-    #_ 
-    #(trivializeable_IIOwp_2 _ _ _ (fun x y h -> pre x y h) post) f) x y
